Rename (term) substitution functions: subst, msubst, etc)

src/PlutusIR/Semantics/Dynamic/Substitution.v
@@ -13,104 +13,104 @@ Local Open Scope string_scope.
 (** Substitution of terms *)
 
 Section SubstBindings.
-  Context {substb : name -> Term -> Binding -> Binding}.
+  Context {subst_b : name -> Term -> Binding -> Binding}.
 
-  Fixpoint substitute_bindings_nonrec (x : name) (s : Term) (bs : list Binding) : list Binding :=
+  Fixpoint subst_bnr' (x : name) (s : Term) (bs : list Binding) : list Binding :=
     match bs with
     | nil => 
         nil
     | b :: bs' => 
         if existsb (eqb x) (bvb b)
           then
-            substb x s b :: bs'
+            subst_b x s b :: bs'
           else
-            substb x s b :: substitute_bindings_nonrec x s bs'
+            subst_b x s b :: subst_bnr' x s bs'
     end.
 
-  Fixpoint substitute_bindings_rec (x : name) (s : Term) (bs : list Binding) : list Binding :=
+  Fixpoint subst_br' (x : name) (s : Term) (bs : list Binding) : list Binding :=
     match bs with
     | nil =>
         nil
     | b :: bs' =>
-        substb x s b :: substitute_bindings_rec x s bs'
+        subst_b x s b :: subst_br' x s bs'
     end.
 
 End SubstBindings.
 
-Fixpoint substitute (x : name) (s : Term) (t : Term) {struct t} : Term :=
+Fixpoint subst (x : name) (s : Term) (t : Term) {struct t} : Term :=
   match t with
   | Let NonRec bs t0 =>
-      Let NonRec (@substitute_bindings_nonrec substitute_binding x s bs)
+      Let NonRec (@subst_bnr' subst_b x s bs)
         (if existsb (eqb x) (bvbs bs) 
           then t0
-          else substitute x s t0
+          else subst x s t0
         ) 
   | Let Rec bs t0 =>
       if existsb (eqb x) (bvbs bs) 
         then 
           Let Rec bs t0
         else
-          Let Rec (@substitute_bindings_rec substitute_binding x s bs) (substitute x s t0)
+          Let Rec (@subst_br' subst_b x s bs) (subst x s t0)
   | Var y => 
       if x =? y
         then s
         else Var y
   | TyAbs bX K t0 =>
-      TyAbs bX K (substitute x s t0)
+      TyAbs bX K (subst x s t0)
   | LamAbs bx T t0 =>
       if x =? bx
         then LamAbs bx T t0
-        else LamAbs bx T (substitute x s t0)
+        else LamAbs bx T (subst x s t0)
   | Apply t1 t2 =>
-      Apply (substitute x s t1) (substitute x s t2)
+      Apply (subst x s t1) (subst x s t2)
   | Constant u =>
       Constant u
   | Builtin d =>
       Builtin d
   | TyInst t0 T =>
-      TyInst (substitute x s t0) T
+      TyInst (subst x s t0) T
   | Error T =>
       Error T
   | IWrap F T t0 =>
-      IWrap F T (substitute x s t0)
+      IWrap F T (subst x s t0)
   | Unwrap t0 =>
-      Unwrap (substitute x s t0)
+      Unwrap (subst x s t0)
   end
 
-with substitute_binding (x : name) (s : Term) (b : Binding) {struct b} : Binding :=
+with subst_b (x : name) (s : Term) (b : Binding) {struct b} : Binding :=
   match b with
   | TermBind stricty (VarDecl y T) tb =>
-      TermBind stricty (VarDecl y T) (substitute x s tb)
+      TermBind stricty (VarDecl y T) (subst x s tb)
   | _ => b
   end.
 
-Definition subst_bnr x s bs := (@substitute_bindings_nonrec substitute_binding x s bs).
-Definition subst_br x s bs := (@substitute_bindings_rec substitute_binding x s bs).
+Definition subst_bnr x s bs := (@subst_bnr' subst_b x s bs).
+Definition subst_br x s bs := (@subst_br' subst_b x s bs).
 
-Notation "'[' s '/' x ']' t" := (substitute x s t) (in custom plutus_term at level 20, x constr).
-Notation "'[' s '/' x '][b]' b" := (substitute_binding x s b) (in custom plutus_term at level 20, x constr).
-Notation "'[' s '/' x '][bnr]' bs" := (@substitute_bindings_nonrec substitute_binding x s bs) (in custom plutus_term at level 20, x constr).
-Notation "'[' s '/' x '][br]' bs" := (@substitute_bindings_rec substitute_binding x s bs) (in custom plutus_term at level 20, x constr).
+Notation "'[' s '/' x ']' t" := (subst x s t) (in custom plutus_term at level 20, x constr).
+Notation "'[' s '/' x '][b]' b" := (subst_b x s b) (in custom plutus_term at level 20, x constr).
+Notation "'[' s '/' x '][bnr]' bs" := (@subst_bnr' subst_b x s bs) (in custom plutus_term at level 20, x constr).
+Notation "'[' s '/' x '][br]' bs" := (@subst_br' subst_b x s bs) (in custom plutus_term at level 20, x constr).
 
 (** Multi-substitutions of terms *)
-Fixpoint msubst_term (ss : list (name * Term)) (t : Term) : Term :=
+Fixpoint msubst (ss : list (name * Term)) (t : Term) : Term :=
   match ss with
   | nil => t
-  | (x, s) :: ss' => msubst_term ss' <{ [s / x] t }>
+  | (x, s) :: ss' => msubst ss' <{ [s / x] t }>
   end.
 
-Fixpoint msubst_binding (ss : list (name * Term)) (b : Binding) : Binding :=
+Fixpoint msubst_b (ss : list (name * Term)) (b : Binding) : Binding :=
   match ss with
   | nil => b
-  | (x, s) :: ss' => msubst_binding ss' <{ [s / x][b] b }>
+  | (x, s) :: ss' => msubst_b ss' <{ [s / x][b] b }>
   end.
 
-Fixpoint msubst_bindings_nonrec (ss : list (name * Term)) (bs : list Binding) : list Binding :=
+Fixpoint msubst_bnr (ss : list (name * Term)) (bs : list Binding) : list Binding :=
   match ss with
   | nil => bs
-  | (x, s) :: ss' => msubst_bindings_nonrec ss' <{ [s / x][bnr] bs }>
+  | (x, s) :: ss' => msubst_bnr ss' <{ [s / x][bnr] bs }>
   end.
 
-Notation "'/[' ss '/]' t" := (msubst_term ss t) (in custom plutus_term at level 20, ss constr).
-Notation "'/[' ss '/][b]' b" := (msubst_binding ss b) (in custom plutus_term at level 20, ss constr).
-Notation "'/[' ss '/][bnr]' bs" := (msubst_bindings_nonrec ss bs) (in custom plutus_term at level 20, ss constr).
+Notation "'/[' ss '/]' t" := (msubst ss t) (in custom plutus_term at level 20, ss constr).
+Notation "'/[' ss '/][b]' b" := (msubst_b ss b) (in custom plutus_term at level 20, ss constr).
+Notation "'/[' ss '/][bnr]' bs" := (msubst_bnr ss bs) (in custom plutus_term at level 20, ss constr).
