src/PlutusIR/Semantics/SemanticEquivalence/Multisubstitution/Congruence.v
@@ -207,7 +207,7 @@ Proof with eauto.
 Qed.
 
 Lemma msubst_LetNonRec_nil : forall ss e,
-    msubst_term ss (Let NonRec nil e) = Let NonRec nil (msubst_term ss e).
+    msubst ss (Let NonRec nil e) = Let NonRec nil (msubst ss e).
 Proof.
   induction ss; intros.
   - reflexivity.
@@ -215,7 +215,7 @@ Proof.
 Qed.
 
 Lemma msubst_LetNonRec : forall ss bs e,
-    msubst_term ss (Let NonRec bs e) = Let NonRec (msubst_bindings_nonrec ss bs) (msubst_term (mdrop (bvbs bs) ss) e).
+    msubst ss (Let NonRec bs e) = Let NonRec (msubst_bnr ss bs) (msubst (mdrop (bvbs bs) ss) e).
 Proof with auto.
   induction ss; intros.
   - rewrite mdrop_nil. reflexivity.
@@ -241,15 +241,15 @@ Proof with auto.
 Qed.
 
 Lemma msubst_TermBind : forall ss stricty x T e,
-    msubst_binding ss (TermBind stricty (VarDecl x T) e) = TermBind stricty (VarDecl x T) (msubst_term ss e). 
+    msubst_b ss (TermBind stricty (VarDecl x T) e) = TermBind stricty (VarDecl x T) (msubst ss e). 
 Proof.
   induction ss; intros.
   - reflexivity.
   - destruct a. eauto.
 Qed.
 
-Lemma msubst_BindingsNonRec_cons : forall ss b bs,
-    msubst_bindings_nonrec ss (b :: bs) = msubst_binding ss b :: msubst_bindings_nonrec (mdrop (bvb b) ss) bs.
+Lemma msubst_bnr_cons : forall ss b bs,
+    msubst_bnr ss (b :: bs) = msubst_b ss b :: msubst_bnr (mdrop (bvb b) ss) bs.
 Proof.
   induction ss; intros.
   - rewrite mdrop_nil. reflexivity.
@@ -310,16 +310,16 @@ Proof.
 (* ADMIT: I had no time to finish this. Should hold, it is a congruence lemma. *)
 Admitted.
 
-Lemma msubst_term__fold : forall ss x v t,
-    msubst_term ss <{ [v / x] t }> = msubst_term ((x, v) :: ss) t.
+Lemma msubst__fold : forall ss x v t,
+    msubst ss <{ [v / x] t }> = msubst ((x, v) :: ss) t.
 Proof. induction ss; intros; auto. Qed.
 
-Lemma msubst_bindings_nonrec__fold : forall ss x v bs,
-    msubst_bindings_nonrec ss <{ [v / x][bnr] bs }> = msubst_bindings_nonrec ((x, v) :: ss) bs.
+Lemma msubst_bnr__fold : forall ss x v bs,
+    msubst_bnr ss <{ [v / x][bnr] bs }> = msubst_bnr ((x, v) :: ss) bs.
 Proof. induction ss; intros; auto. Qed.
 
 Lemma msubst_LamAbs : forall ss x T t0,
-    msubst_term ss (LamAbs x T t0) = LamAbs x T (msubst_term (drop x ss) t0).
+    msubst ss (LamAbs x T t0) = LamAbs x T (msubst (drop x ss) t0).
 Proof.
   induction ss; intros.
   - reflexivity.
@@ -347,7 +347,7 @@ Proof.
 Qed.
 
 Lemma msubst_Apply : forall ss t1 t2,
-    msubst_term ss (Apply t1 t2) = Apply (msubst_term ss t1) (msubst_term ss t2).
+    msubst ss (Apply t1 t2) = Apply (msubst ss t1) (msubst ss t2).
 Proof.
   induction ss; intros.
   - reflexivity.
@@ -363,7 +363,7 @@ Proof.
 Qed.
 
 Lemma msubst_Builtin : forall ss f,
-    msubst_term ss (Builtin f) = Builtin f.
+    msubst ss (Builtin f) = Builtin f.
 Proof. 
   induction ss; intros.
   - reflexivity.
@@ -379,7 +379,7 @@ Proof.
 Qed.
 
 Lemma msubst_Constant : forall ss sv,
-    msubst_term ss (Constant sv) = Constant sv.
+    msubst ss (Constant sv) = Constant sv.
 Proof.
   induction ss; intros. 
   - reflexivity.
@@ -404,7 +404,7 @@ Proof.
 Qed.
 
 Lemma msubst_DatatypeBind : forall ss X YKs matchFunc cs,
-    msubst_binding ss (DatatypeBind (Datatype X YKs matchFunc cs)) = DatatypeBind (Datatype X YKs matchFunc cs).
+    msubst_b ss (DatatypeBind (Datatype X YKs matchFunc cs)) = DatatypeBind (Datatype X YKs matchFunc cs).
 Proof.
   induction ss; intros.
   - reflexivity.
@@ -421,7 +421,7 @@ Qed.
 
 
 Lemma msubst_Error : forall ss T,
-    msubst_term ss (Error T) = Error T.
+    msubst ss (Error T) = Error T.
 Proof. 
   induction ss; intros.
   - reflexivity.
@@ -437,7 +437,7 @@ Proof.
 Qed.
 
 Lemma msubst_IWrap : forall ss F T M,
-    msubst_term ss (IWrap F T M) = IWrap F T (msubst_term ss M).
+    msubst ss (IWrap F T M) = IWrap F T (msubst ss M).
 Proof. 
   induction ss; intros.
   - reflexivity.
@@ -461,7 +461,7 @@ Proof.
 Qed. 
 
 Lemma msubst_TyAbs : forall ss bX K t0,
-    msubst_term ss (TyAbs bX K t0) = TyAbs bX K (msubst_term ss t0).
+    msubst ss (TyAbs bX K t0) = TyAbs bX K (msubst ss t0).
 Proof. induction ss; intros. - reflexivity. - destruct a. eauto. Qed.
 
 Lemma msubstA_TyAbs : forall ss bX K t0,
@@ -474,7 +474,7 @@ Lemma msubstT_TyForall : forall ss bX K T,
 Proof. induction ss; intros. - reflexivity. - intros. destruct a. simpl. destruct (s =? bX)%string; eauto. Qed.
 
 Lemma msubst_TyInst : forall ss t0 T0,
-    msubst_term ss (TyInst t0 T0) = TyInst (msubst_term ss t0) T0.
+    msubst ss (TyInst t0 T0) = TyInst (msubst ss t0) T0.
 Proof. induction ss; intros. - reflexivity. - destruct a. eauto. Qed.
 
 
@@ -484,7 +484,7 @@ Proof. induction ss; intros. - reflexivity. - destruct a. eauto. Qed.
 
 
 Lemma msubst_Unwrap : forall ss M,
-    msubst_term ss (Unwrap M) = Unwrap (msubst_term ss M).
+    msubst ss (Unwrap M) = Unwrap (msubst ss M).
 Proof. induction ss; intros. - reflexivity. - destruct a. eauto. Qed.
 
 Lemma msubstA_Unwrap : forall ss M ,
@@ -494,7 +494,7 @@ Proof. induction ss; intros. - reflexivity. - destruct a. eauto. Qed.
 
 Lemma msubst_Var : forall ss x,
     closed_env ss ->
-    msubst_term ss (Var x) =
+    msubst ss (Var x) =
       match lookup x ss with
       | Datatypes.Some t => t
       | None => Var x
